\usetypescriptfile[type-xits]
\usetypescript[xits]
\setupbodyfont[xits]

\setuplayout[header=0pt,footer=0pt]
\setupformulas[spaceafter={2*big}]

\starttext

\midaligned{$\bfd\frak XITS\ Math$}\blank[4*big]

\startformula
\pi(n) = \sum^{n}_{m=2}\left\lfloor\biggl(\sum^{m-1}_{k=1}\bigl\lfloor(m/k)\big/\lceil m/k\rceil\bigr\rfloor\biggr)^{-1}\right\rfloor
\stopformula

\startformula
\pi(n) = \sum^{n}_{k=2}\left\lfloor\phi(k) \over k-1\right\rfloor
\stopformula

\startformula
1+\left(1\over1-x^2\right)^3
\stopformula

\startformula
1+\left(1\over1-{{{x^2}\over{y^3}}\over{z^4}}\right)^3
\stopformula

\startformula
{a+1\over b}\bigg/{c+1\over d}
\stopformula

\startformula
\biggl({\partial^{2} \over \partial x^{2}} + {\partial^{2} \over \partial y^{2}}\biggr) {\bigl\vert\phi(x+iy)\bigr\vert}^2
\stopformula

\startformula
\sum_{\scriptstyle0\le i\le m\atop\scriptstyle0<j<n}P(i,j)
\stopformula

\startformula
\int_0^3 9x^2 + 2x + 4\, dx = 3x^3 + x^2 + 4x + C \Big]_0^3 = 102
\stopformula

\startformula
e^{x+iy} = e^x(\cos y + i\sin y)
\stopformula

\startformula
x = {-b \pm \sqrt{b^2 - 4ac} \over 2a}
\stopformula

\startformula
 f(x) = 
   \startmathcases
     \NC x, \MC \text{if } 0 \le x \le \frac12 \NR
     \NC 1-x ,\MC \text{if } \frac12 \le x \le 1 \NR
   \stopmathcases
\stopformula

\startformula
\sqrt{1+\sqrt{1+\sqrt{1+\sqrt{1+\sqrt{1+\sqrt{1+\sqrt{1+x}}}}}}}
\stopformula

\startformula
{\bf S^{\rm -1} TS} = {\bf dg}(\omega_1,\ldots,\omega_n) = {\bf \Lambda}
\stopformula

\startformula
\Pr(\,m=n\mid m+n=3\,)
\stopformula

\startformula
\sin 18^\circ = {1\over 4} (\sqrt{5}-1)
\stopformula

\startformula
k=1.38 \times 10^{-16}\,\rm erg/^\circ K
\stopformula

\startformula
\bar\Phi \subset NL^*_1/N=\bar L^*_1\subseteq\cdots\subseteq  NL^*_n/N=\bar L^*_n
\stopformula

\startformula
\textstyle I(\lambda)=\iint_D g(x,y)e^{i\lambda h(x,y)}\,dx\, dy
\stopformula

\startformula
\textstyle\int^1_0\cdots\int^1_0 f(x_1,\ldots,x_n)\, dx_1\ldots dx_n
\stopformula

\startformula
x_{2m} \equiv \cases{Q(X^2_m - P_2W^2_m)-2S^2 & ($m$ odd)\cr
                     &\cr
                     P^2_2(X^2_m - P_2W^2_m)-2S^2 & ($m$ even)} \pmod N
\stopformula

\startformula
(1+x_1z+x^2_1z^2+\cdots\,)\ldots(1+x_nz+x^2_nz^2+\cdots\,)={1\over(1-x_1z)\ldots(1-x_nz)}
\stopformula

\startformula
\prod_{j\ge 0}\biggl(\sum_{k\ge0}a_{jk}z^k\biggr) =
\sum_{n\ge 0} z^n \Biggl(\sum_{k_0,k_1,\ldots\ge 0\atop k_0+k_1+\cdots=n} a_{0k_0}a_{1k_1}\ldots\,\Biggr)
\stopformula

\startformula
\sum^\infty_{n=0} a_nz^n\qquad\hbox{converges if}\qquad|z|\lt\left(\limsup_{n\to\infty} \root n \of {|a-n|}\right)
\stopformula

\startformula
{f(x+\Delta x)-f(x)\over\Delta x}\to f'(x)\qquad\hbox{as $\Delta x\to 0$}
\stopformula

\startformula
\Vert u_i\Vert = 1, \qquad u_i\cdot u_j = 0 \quad\hbox{if $i\neq j$}
\stopformula

\startformula
\prod_{k\ge0}{1\over(1-q^kz)}=\sum_{n\ge0}z^n\bigg/\!\!\prod_{1\le k\le n}(1-q^k).\eqno(16')
\stopformula

\startformula
\eqalign{T(n)\le T(2^{\lceil\lg n\rceil})&\le c(3^{\lceil\lg n\rceil}-2^{\lceil\lg n\rceil})\cr
                                         &< 3c\cdot3^{\lg n}\cr
                                         &= 3cn^{\lg n}}
\stopformula

\startformula
\eqalign{P(x)&=a_0+a_1x+a_2x^2+\cdots+a_nx^2,\cr
        P(-x)&=a_0-a_1x+a_2x^2-\cdots+(-1)^na_nx^2.}
\eqno(30)
\stopformula

\startformula
\leqalignno{\gcd(u,v)&=\gcd(v,u); &(9)\cr
            \gcd(u,v)&=\gcd(-u,v).&(10)}
\stopformula

\startformula
\reqalignno{
\biggl(\int^\infty_{-\infty}e^{-x^2}dx\biggr)^2 & =\int^\infty_{-\infty}\int^\infty_{-\infty}e^{-(x^2+y^2)}\,dx\,dy\cr
                                                & =\int^{2\pi}_0\int^\infty_0 e^{-r^2} r\,dr\,d\theta\cr
                                                & =\int^{2\pi}_0\biggl(-{e^{-r^2}\over2}\bigg|^{r=\infty}_{r=0}\,\biggr)\,d\theta\cr
                                                & =\pi.&(11)
}
\stopformula

\stoptext
